pretty.v
@@ -1,0 +1,126 @@
+Require Import EqNat.
+
+Inductive code : Set :=
+  | I : code
+  | K : code
+  | B : code
+  | C : code
+  | W : code
+  | S : code
+  | J : code
+  | BOT : code
+  | TOP : code
+  | AP : code -> code -> code.
+
+Inductive Term {extend : Set} : Set :=
+  | VAR: nat -> Term
+  | APP: Term -> Term -> Term
+  | ABS: nat -> Term -> Term
+  | DEF: nat -> Term -> Term -> Term
+  | ERROR: Term
+  | HOLE: Term
+  | JOIN: Term -> Term -> Term
+  | INLINE: extend -> Term.
+
+Definition term_ (e : Set) := Term (extend := e).
+Definition term := term_ Empty_set.
+Definition term' := term_ code.
+
+(** The [term_] monad *)
+Definition inline (a : Set) : a -> term_ a := fun x => INLINE x.
+Fixpoint coerce {a b : Set} (f : a -> term_ b) (x : term_ a) : term_ b :=
+  match x with
+  | VAR n => VAR n
+  | APP x0 x1 => APP (coerce f x0) (coerce f x1)
+  | ABS n x0 => ABS n (coerce f x0)
+  | DEF n x0 x1 => DEF n (coerce f x0) (coerce f x1)
+  | ERROR => ERROR
+  | HOLE => HOLE
+  | JOIN x0 x1 => JOIN (coerce f x0) (coerce f x1)
+  | INLINE x0 => f x0
+  end.
+
+Definition var (n : nat) : term := VAR n.
+Definition app (x y : term) := APP x y.
+Definition abs (x y : term) : term :=
+  match x with
+  | VAR n => ABS n y
+  | z => HOLE
+  end.
+Definition join (x y : term) := JOIN x y.
+Definition error : term := ERROR.
+Definition hole : term := HOLE.
+
+
+Section Encode.
+  Notation "[ x ]" := (INLINE x).
+  Notation "x [*] y" := (APP x y) (at level 40, left associativity).
+
+  Fixpoint occurs (n : nat) (x : term') : bool :=
+    match x with
+    | VAR n0 => beq_nat n n0
+    | APP x0 x1 => orb (occurs n x0) (occurs n x1)
+    | ABS n0 x0 => andb (negb (beq_nat n n0)) (occurs n x0)
+    | JOIN x0 x1 => orb (occurs n x0) (occurs n x1)
+    | _ => false
+    end.
+
+  (* TODO implement prettier abstraction *)
+  Fixpoint abstract (n : nat) (x : term') : term' :=
+    match x with
+    | VAR m => if beq_nat m n then [I] else [K] [*] (VAR m)
+    | ABS m y =>
+        if beq_nat m n
+        then [K] [*] (ABS m y)
+        else ABS m (abstract n y)
+    | DEF m y z =>
+        if beq_nat m n
+        then [K] [*] (DEF m y z)
+        else ERROR (* TODO *)
+    | APP y z => [S] [*] (abstract n y) [*] (abstract n z)
+    | JOIN y z => [J] [*] (abstract n y) [*] (abstract n z)
+    | y => [K] [*] y
+    end.
+
+  Fixpoint compile (x : term') : term' :=
+    match x with
+    | APP y z => APP (compile y) (compile z)
+    | ABS n y => abstract n (compile y)
+    | y => y
+    end.
+
+  Fixpoint close (x : term') : code :=
+    match x with
+    | INLINE y => y
+    | APP y z => AP (close y) (close z)
+    | _ => TOP
+    end.
+
+  Definition noop (x : Empty_set) : term' := match x with end.
+  Definition encode (x : term) : code := close(compile(coerce noop x)).
+End Encode.
+
+Section combinators.
+  Notation "\ x , y" := (abs x y) (at level 60, right associativity).
+  Notation "x 'o' y" := (app x y) (at level 35, right associativity).
+  Notation "x * y" := (app x y) (at level 40, left associativity).
+  Notation "x || y" := (join x y) (at level 50, left associativity).
+
+  Let x := var 0.
+  Let y := var 1.
+  Let z := var 2.
+
+  Definition TOP' := error.
+  Definition S' := \x,\y,\z, x*z*(y*z).
+  Definition K' := \x,\y, x.
+  Definition I' := \x, x.
+  Definition B' := \x,\y,\z, x*(y*z).
+  Definition C' := \x,\y,\z, x*z*y.
+  Definition Y' := \x, (\y, x*(y*y)) * (\y, x*(y*y)).
+  Definition V' := Y' * \x,\y, I' || x o y.
+  Definition div' := Y' * \x, x * TOP'.
+
+  Definition Y := encode Y'.
+  Definition V := encode V'.
+  Definition div := encode div'.
+End combinators.
