sampling.v
@@ -1,4 +1,0 @@
-
-Require Import Coq.Structures.Orders.
-
-Inductive Random (Omega : Set) (A : Set) : Set := TODO.
